refactor: use Imperative_HOL directly and override the module code

src/IO.thy
@@ -1,14 +1,14 @@
 theory IO
-  imports Main "HOL-Imperative_HOL.Array"
+  imports Main "HOL-Imperative_HOL.Imperative_HOL"
 begin
 
 datatype 'a io = IO (run_io: "'a Heap")
 
 definition return :: "'a \<Rightarrow> 'a io" where
-  "return x = IO (Heap_Monad.return x)"
+  [code del]: "return x = IO (Heap_Monad.return x)"
 
 definition bind :: "'a io \<Rightarrow> ('a \<Rightarrow> 'b io) \<Rightarrow> 'b io" where
-  "bind x f = IO (Heap_Monad.bind (run_io x) (run_io \<circ> f))"
+  [code del]: "bind x f = IO (Heap_Monad.bind (run_io x) (run_io \<circ> f))"
 
 adhoc_overloading
   Monad_Syntax.bind IO.bind
@@ -28,54 +28,6 @@ lemma monad_assoc[simp]:
   shows "(m \<bind> f) \<bind> g = m \<bind> (\<lambda>x. f x \<bind> g)"
   unfolding bind_def comp_def by (auto split: prod.splits)
 
-definition present_heap :: "heap \<Rightarrow> 'a::heap ref \<Rightarrow> bool" where
-  "present_heap h r \<longleftrightarrow> addr_of_ref r < lim h"
-
-definition get_heap :: "heap \<Rightarrow> 'a::heap ref \<Rightarrow> 'a" where
-  "get_heap h = from_nat \<circ> refs h TYPEREP('a) \<circ> addr_of_ref"
-
-definition set_heap :: "'a::heap ref \<Rightarrow> 'a \<Rightarrow> heap \<Rightarrow> heap" where
-  "set_heap r x = refs_update
-    (\<lambda>h. h(TYPEREP('a) := ((h (TYPEREP('a))) (addr_of_ref r := to_nat x))))"
-
-definition alloc_heap_array :: "nat \<Rightarrow> heap \<Rightarrow> 'a::heap array \<times> heap" where
-  "alloc_heap_array s h = (let
-     l = lim h;
-     r = Array l
-   in (r, (h\<lparr>lim := l + s\<rparr>)))"
-
-definition alloc_heap :: "'a \<Rightarrow> heap \<Rightarrow> 'a::heap ref \<times> heap" where
-  "alloc_heap v h = (let
-     l = lim h;
-     r = Ref l
-   in (r, set_heap r v (h\<lparr>lim := l + 1\<rparr>)))"
-
-definition noteq :: "'a::heap ref \<Rightarrow> 'b::heap ref \<Rightarrow> bool" (infix "=!=" 70) where
-  "r =!= s \<longleftrightarrow> TYPEREP('a) \<noteq> TYPEREP('b) \<or> addr_of_ref r \<noteq> addr_of_ref s"
-
-definition alloc :: "nat \<Rightarrow> 'a::heap array io" where
-  "alloc s = IO (Heap_Monad.heap (alloc_heap_array s))"
-
-definition ref :: "'a::heap \<Rightarrow> 'a ref io" where
-  [code del]: "ref v = IO (Heap_Monad.heap (alloc_heap v))"
-
-definition lookup :: "'a::heap ref \<Rightarrow> 'a io" ("!_" 61) where
-  [code del]: "lookup r = IO (Heap_Monad.tap (\<lambda>h. get_heap h r))"
-
-definition update :: "'a ref \<Rightarrow> 'a::heap \<Rightarrow> unit io" ("_ := _" 62) where
-  [code del]: "update r v = IO (Heap_Monad.heap (\<lambda>h. ((), set_heap r v h)))"
-
-definition modify :: "('a::heap \<Rightarrow> 'a) \<Rightarrow> 'a ref \<Rightarrow> 'a io" where
-  "modify f r = do {
-     x \<leftarrow> ! r;
-     let y = f x;
-     r := y;
-     return y
-   }"
-
-primrec extract_io :: "'a io \<Rightarrow> heap \<Rightarrow> 'a option" where
-  "extract_io (IO v) h = map_option fst (execute v h)"
-
 (* Monadic Combinators *)
 
 fun forMu :: "'a list \<Rightarrow> ('a \<Rightarrow> unit io) \<Rightarrow> unit io" where
@@ -91,27 +43,6 @@ fun whenu :: "bool \<Rightarrow> unit io \<Rightarrow> unit io" where
 
 fun whenM :: "bool io \<Rightarrow> unit io \<Rightarrow> unit io" where
   "whenM cond f = cond \<bind> (\<lambda>b. if b then f else return ())"
-
-(*
-code_printing
-  type_constructor io \<rightharpoonup> (Haskell) "IO _"
-  | type_constructor ref \<rightharpoonup> (Haskell) "IORef _"
-  | type_constructor array \<rightharpoonup> (Haskell) "V.IOVector _"
-  | constant return \<rightharpoonup> (Haskell) "return"
-  | constant ref \<rightharpoonup> (Haskell) "newIORef"
-  | constant look \<rightharpoonup> (Haskell) "readIORef"
-  | constant put \<rightharpoonup> (Haskell) "writeIORef"
-  | constant new_array \<rightharpoonup> (Haskell) "V.unsafeNew"
-  | constant read_array \<rightharpoonup> (Haskell) "unsafeRead"
-  | constant write_array \<rightharpoonup> (Haskell) "unsafeWrite"
-  | constant swap_array \<rightharpoonup> (Haskell) "unsafeSwap"
-  | constant forMu \<rightharpoonup> (Haskell) "forM_"
-  | constant mapM \<rightharpoonup> (Haskell) "mapM_"
-  | constant whenu \<rightharpoonup> (Haskell) "when"
-*)
-
-lemma set_set_heap [simp]: "set_heap r v2 (set_heap r v1 h) = set_heap r v2 h"
-  by (simp add: set_heap_def)
 
 definition execute_io where
   "execute_io c h = execute (run_io c) h"
@@ -130,19 +61,16 @@ qed
 lemma io_bind_execute[simp]: "execute_io (m \<bind> k) h = (execute_io m h) \<bind> (\<lambda>(val,h'). execute_io (k val) h')"
   by (simp add: IO.bind_def execute_io_def)
 
-lemma execute_alloc: "execute_io (alloc n) h = (let l = lim h in Some (Array l, h \<lparr> lim := l + n \<rparr>))"
-  apply (simp add: execute_io_def alloc_def heap_def alloc_heap_array_def)
-  apply metis
-  done
+code_printing code_module "IO" \<rightharpoonup> (Haskell)
+\<open>import qualified Data.Vector\<close>
 
-lemma execute_update: "execute_io (r := v) h = Some ((), (set_heap r v h))"
-  by (simp add: update_def effect_io_def execute_io_def heap_def)
+code_printing code_module "Heap" \<rightharpoonup> (Haskell)
 
-lemma effect_update: "effect_io (r := v) h (set_heap r v h) ()"
-  by (simp add: update_def effect_io_def execute_io_def heap_def)
-
-lemma update_update: "execute_io (update r v1 \<bind> (\<lambda>_. update r v2)) h = execute_io (update r v2) h"
-  by (simp add: execute_update)
-
+code_printing
+  type_constructor io \<rightharpoonup> (Haskell) "IO _"
+  | type_constructor ref \<rightharpoonup> (Haskell) "IORef _"
+  | type_constructor array \<rightharpoonup> (Haskell) "V.IOVector _"
+  | constant return \<rightharpoonup> (Haskell) "return"
+  | constant bind \<rightharpoonup> (Haskell) infixl 5 ">>="
 
 end
